rename img_lat, real_lat into lat_img, lat_real

theories/modules/FSpec.v
@@ -75,7 +75,7 @@ Section FSPEC.
     postcondS := λ '(existT i meta_i), (nth i fspecs fspecS_bot).(postcondS) meta_i
   |}.
 
-  Definition img_lat_body (peeking: bool) (fsp : fspecS) (lbody: itree crisE ()) (body: fbody) (arg: Any.t) :=
+  Definition lat_img_body (peeking: bool) (fsp : fspecS) (lbody: itree crisE ()) (body: fbody) (arg: Any.t) :=
     lbody;;;
     x <- trigger (Take (metaS fsp));;
     trigger (Assume (precondS fsp x arg));;;
@@ -86,10 +86,10 @@ Section FSPEC.
          (if b then peek else update)
     else update.
 
-  Definition img_lat peeking fsp lbody body : fbody :=
-    λ arg, ITree.iter (λ _, img_lat_body peeking fsp lbody body arg) ().
+  Definition lat_img peeking fsp lbody body : fbody :=
+    λ arg, ITree.iter (λ _, lat_img_body peeking fsp lbody body arg) ().
 
-  Definition real_lat_body (peeking: bool) (fsp : fspecS) (lbody: itree crisE ()) (body: fbody) (arg: Any.t) :=
+  Definition lat_real_body (peeking: bool) (fsp : fspecS) (lbody: itree crisE ()) (body: fbody) (arg: Any.t) :=
     lbody;;;
     let peek := RealUpdate (λ x, precondS fsp x arg) (λ x, precondS fsp x arg);;; Ret (inl ()) in
     let update := ret <- body arg;; RealUpdate (λ x, precondS fsp x arg) (λ x, postcondS fsp x ret);;; Ret (inr ret) in
@@ -98,8 +98,8 @@ Section FSPEC.
          (if b then peek else update)
     else update.
 
-  Definition real_lat peeking fsp lbody body : fbody :=
-    λ arg, ITree.iter (λ _, real_lat_body peeking fsp lbody body arg) ().
+  Definition lat_real peeking fsp lbody body : fbody :=
+    λ arg, ITree.iter (λ _, lat_real_body peeking fsp lbody body arg) ().
 
   Definition to_fspec (fsp : fspecS) : fspec :=
     mk_fspec (λ x varg arg, (fsp.(precondS) x arg ∗ ⌜varg = arg⌝)%I)
